\begin{algorithm}\label{alg:1}
       \caption{EMTLe}\label{alg:1}
        \begin{algorithmic}[1]
            \REQUIRE $\lambda, \psi,Y,f',T$,
            \ENSURE $\beta=\left\{\beta^1,...,\beta^n\right\}$
            \STATE $\beta^0 = 1$
            ,$\alpha' = \psi^{-1}Y,\alpha'' = \psi^{-1}f'$
            \FOR {$t=1$ to $T$}
                \STATE $\hat Y \leftarrow Y - {\left( {\psi^{-1} \circ I} \right)^{ - 1}}\left( \alpha' - \alpha''diag(\beta) \right)$
                %\STATE ${\Delta _\beta }=0$ 
                \FOR {$i=1$ to $l$}
                	\STATE ${\Delta _\beta }=\lambda\beta$ 
                	%\FOR {$r=1$ to $N$}
	                    \STATE $l_{ir} = \max(1 - {\varepsilon _{{y_i}r}} + {\hat Y_{ir}} - {\hat Y_{i{y_i}}})$
	                    \IF{$l_{ir}>0$}
	                            \STATE $\Delta _\beta^{{y_i}} \leftarrow \Delta _\beta^{{y_i}} - \frac{{{\alpha''_{i{y_i}}}}}{{{\psi^{-1}_{ii}}}}$%
	                            , $\Delta _\beta^{{r}} \leftarrow \Delta _\beta^{{r}} + \frac{{{\alpha''_{i{r}}}}}{{{\psi^{-1}_{ii}}}}$%
	                    \ENDIF
	                 %\ENDFOR %class ends   
                \ENDFOR %examples ends
                \STATE $\beta^t  \leftarrow \beta^{(t-1)}  - \frac{{{\Delta _\beta }}}{{\lambda\times {t} }}$
             \ENDFOR %iteration ends
        \end{algorithmic}
\end{algorithm}